---
{"dg-publish":true,"permalink":"/math/implicit-differentiation/"}
---


When we do not have $y$ explicitly as a function of $x$, example for $x^2+y^2=1$

	$$\frac{d}{dx}(x^2+y^2)=\frac{d}{dx}(1)$$
	$$\implies \frac{d}{dx}x^2+\frac{d}{dx}y^2=0$$
	$$\implies 2x+\frac{d}{dx}y^2=0$$
	$$\implies2x+2y\frac{dy}{dx}=0$$
	
Rearranging this equation, we obtain: 
$$\frac{dy}{dx}=\frac{-x}{y}$$
#### Differentiating $y^2$ with respect to $x$

Let $y^2$ = v, then we have 
$$\frac{d}{dx}y^2=\frac{d}{dx}v=\frac{dv}{dx}=\frac{dv}{dy}\times \frac{dy}{dx}$$
